src/AuxRel.v
@@ -1,0 +1,214 @@
+From imm Require Import Events Execution imm_s_hb.
+From imm Require Import imm_s_ppo.
+From imm Require Import imm_s_hb.
+From imm Require Import imm_bob.
+From imm Require Import SubExecution.
+
+Require Import Program.Basics.
+
+From PromisingLib Require Import Language Basic.
+From hahn Require Import Hahn.
+From hahn Require Import HahnTrace.
+From hahn Require Import HahnSorted.
+From hahnExt Require Import HahnExt.
+From imm Require Import Events Execution Execution_eco imm_s_hb.
+From imm Require Import imm_s_ppo.
+From imm Require Import imm_s_hb.
+From imm Require Import imm_bob.
+From imm Require Import SubExecution.
+From imm Require Import CombRelations.
+
+Section AuxRel.
+
+Variable G : execution.
+Notation "'lab'" := (lab G).
+Notation "'E'" := (acts_set G).
+Notation "'loc'" := (loc lab).
+Notation "'same_loc'" := (same_loc lab).
+Notation "'is_acq'" := (is_acq lab).
+Notation "'is_rel'" := (is_rel lab).
+Notation "'is_rlx'" := (is_rlx lab).
+Notation "'sb'" := (sb G).
+Notation "'rf'" := (rf G).
+Notation "'co'" := (co G).
+Notation "'rmw'" := (rmw G).
+Notation "'ppo'" := (ppo G).
+Notation "'hb'" := (hb G).
+Notation "'psc'" := (imm.psc G).
+Notation "'sw'" := (sw G).
+Notation "'W'" := (is_w lab).
+Notation "'R'" := (is_r lab).
+Notation "'F'" := (is_f lab).
+Notation "'bob'" := (bob G).
+
+Definition ppo_alt := (sb ∩ same_loc ∪ bob)⁺.
+Definition hb_alt := (ppo_alt ∪ rf)⁺.
+Definition rpo :=
+  sb ∩ same_loc ∪
+  ⦗is_acq⦘ ⨾ sb ⨾ ⦗is_rel⦘ ∪
+  ⦗R ∩₁ is_rlx⦘ ⨾ sb ⨾ ⦗F ∩₁ is_acq⦘ ∪
+  ⦗is_acq⦘ ⨾ sb ⨾ ⦗R ∪₁ W⦘ ∪
+  ⦗R ∪₁ W⦘ ⨾ sb ⨾ ⦗is_rel⦘ ∪
+  ⦗F ∩₁ is_rel⦘ ⨾ sb ⨾ ⦗W ∩₁ is_rlx⦘.
+Definition rhb := (rpo ∪ sw)⁺.
+Definition vf := ⦗E⦘ ⨾ ⦗W⦘ ⨾ rf^? ⨾ hb^? ⨾ psc^? ⨾ hb^?.
+Definition srf := (vf ∩ same_loc) ⨾ ⦗R⦘ \ (co ⨾ vf).
+
+Lemma rpo_in_sb : rpo ⊆ sb.
+Proof using.
+  unfold rpo. unfolder. ins. desf.
+Qed.
+
+Lemma wf_rpoE
+    (WF : Wf G) :
+  rpo ≡ ⦗E⦘ ⨾ rpo ⨾ ⦗E⦘.
+Proof using.
+  split; [| basic_solver].
+  unfolder. intros x y REL.
+  splits; ins.
+  all: apply rpo_in_sb in REL.
+  all: unfold sb in REL; unfolder in REL; desf.
+Qed.
+
+Lemma wf_vfE
+    (WF : Wf G) :
+  vf ≡ ⦗E⦘ ⨾ vf. (* TODO: vf is actually E -> E *)
+Proof using.
+  split; [| basic_solver].
+  unfold vf. hahn_frame.
+  seq_rewrite <- !(id_inter E E).
+  now rewrite !set_interK.
+Qed.
+
+Lemma vf_dom : dom_rel vf ⊆₁ W.
+Proof using.
+  unfold vf. basic_solver.
+Qed.
+
+Lemma wf_srfE
+    (WF : Wf G) :
+  srf ≡ ⦗E⦘ ⨾ srf. (* TODO: srf is actually E -> E *)
+Proof using.
+  split; [| basic_solver]. unfold srf.
+  rewrite wf_vfE at 1 by auto.
+  rewrite seq_eqv_inter_ll, seqA.
+  basic_solver.
+Qed.
+
+Lemma wf_srfD : srf ≡ ⦗W⦘ ⨾ srf ⨾ ⦗R⦘.
+Proof using.
+  split; [| basic_solver]. unfold srf.
+  intros x y SRF. unfolder in SRF. desf.
+  unfolder; ins; desf; splits; ins.
+  { apply vf_dom. now exists y. }
+  exists y; ins.
+Qed.
+
+Lemma wf_srf_loc : srf ⊆ same_loc.
+Proof using.
+  unfold srf. intros x y SRF.
+  unfolder in SRF; desf.
+Qed.
+
+Lemma wf_rhbE
+    (WF : Wf G) :
+  rhb ≡ ⦗E⦘ ⨾ rhb ⨾ ⦗E⦘.
+Proof using.
+  unfold rhb. rewrite wf_swE, wf_rpoE; auto.
+  rewrite <- seq_union_r, <- seq_union_l.
+  seq_rewrite <- ct_seq_eqv_l.
+  rewrite <- seqA.
+  now seq_rewrite <- ct_seq_eqv_r.
+Qed.
+
+Lemma rf_sub_vf (WF : Wf G) : rf ⊆ vf.
+Proof using.
+  rewrite WF.(wf_rfD), WF.(wf_rfE).
+  unfold vf; unfolder; ins; desf.
+  splits; eauto.
+  do 3 (exists y; splits; eauto).
+Qed.
+
+Lemma wf_srff (WF : Wf G) : functional srf⁻¹.
+Proof using.
+  unfolder; unfold srf. intros x y z (VF1 & CO1) (VF2 & CO2).
+  tertium_non_datur (y = z) as [EQ|NEQ]; ins; exfalso.
+  destruct WF.(wf_co_total) with (a := y) (b := z)
+                                 (ol := loc x) as [CO|CO].
+  all: ins; unfolder in *; desf; splits; eauto.
+  all: try now (apply vf_dom; eexists; eauto).
+  { apply wf_vfE in VF1; unfolder in VF1; desf. }
+  apply wf_vfE in VF2; unfolder in VF2; desf.
+Qed.
+
+(* TODO: this is limited to E, which is bad. *)
+Lemma srf_exists b
+    (HIN : E b)
+    (FIN_ACTS : set_finite E)
+    (WF : Wf G)
+    (IS_R : R b) :
+  exists a, srf a b.
+Proof using.
+  assert (HLOC : exists l, loc b = Some l); desf.
+  { unfold is_r in IS_R. unfold loc. desf. eauto. }
+  assert (HINIT : E (InitEvent l)).
+  { apply WF; eauto. }
+  assert (INILAB : lab (InitEvent l) = Astore Xpln Opln l 0).
+  { apply WF. }
+  assert (INILOC : loc (InitEvent l) = Some l).
+  { unfold loc. now rewrite (wf_init_lab WF). }
+  assert (INIW : W (InitEvent l)).
+  { unfold is_w, loc. desf. }
+  assert (INISB : sb (InitEvent l) b).
+  { eapply init_ninit_sb, read_or_fence_is_not_init; eauto. }
+  assert (INIVF : vf (InitEvent l) b).
+  { unfold vf. exists (InitEvent l).
+    splits; ins.
+    hahn_rewrite <- sb_in_hb.
+    basic_solver 21. }
+  assert (ACT_LIST : exists El, E ≡₁ (fun x => In x El)); desf.
+  { apply set_finiteE in FIN_ACTS. desf. eauto. }
+  forward (eapply last_exists with (s:= co ⨾ ⦗fun x => vf x b⦘)
+                                   (dom := filterP W El)
+                                   (a := InitEvent l)).
+  { eapply acyclic_mon.
+    apply trans_irr_acyclic; [apply co_irr | apply co_trans]; eauto.
+    basic_solver. }
+  { ins.
+    assert (A: (co ⨾ ⦗fun x : actid => vf x b⦘)^? (InitEvent l) c).
+    { apply rt_of_trans; try done.
+      apply transitiveI.
+      arewrite_id ⦗fun x : actid => vf x b⦘ at 1.
+      rewrite seq_id_l.
+      arewrite (co ⨾ co ⊆ co); [|done].
+      apply transitiveI.
+      eapply co_trans; eauto. }
+    unfolder in A; desf.
+    { apply in_filterP_iff; split; auto.
+      by apply ACT_LIST. }
+    apply in_filterP_iff.
+    hahn_rewrite WF.(wf_coE) in A.
+    hahn_rewrite WF.(wf_coD) in A.
+    hahn_rewrite WF.(wf_col) in A.
+    unfold same_loc in *; unfolder in *; desf; splits; eauto; congruence. }
+  ins; desc.
+  assert (A: (co ⨾ ⦗fun x : actid => vf x b⦘)^? (InitEvent l) b0).
+  { apply rt_of_trans; [|by subst].
+    apply transitiveI.
+    arewrite_id ⦗fun x : actid => vf x b⦘ at 1.
+    rewrite seq_id_l.
+    arewrite (co ⨾ co ⊆ co); [|done].
+    apply transitiveI.
+    eapply co_trans; eauto. }
+  assert (loc b0 = Some l).
+  { unfolder in A; desf.
+    hahn_rewrite WF.(wf_col) in A.
+    unfold same_loc in *; desf; unfolder in *; congruence. }
+  exists b0; red; split.
+  { unfold urr, same_loc.
+    unfolder in A; desf; unfolder; ins; desf; splits; try basic_solver 21; congruence. }
+  unfold max_elt in *.
+  unfolder in *; ins; desf; intro; desf; basic_solver 11.
+Qed.
+
+End AuxRel.
